code/gf128/Hacl.Spec.GF128.PolyLemmas.fsti
@@ -2,6 +2,7 @@ module Hacl.Spec.GF128.PolyLemmas
 
 open FStar.Mul
 
+open Lib.IntTypes
 open Lib.IntVector
 
 open Vale.Math.Poly2_s
@@ -52,4 +53,24 @@ val lemma_vec128_double_shift (a:poly) : Lemma
     let q = to_vec128 a in
     q <<| 64ul == to_vec128 (mul (mod a (monomial 64)) (monomial 64)) /\
     q >>| 64ul == to_vec128 (div a (monomial 64))
+  ))
+
+val lemma_vec128_shift_left_64 (p:vec128) (s:shiftval U64) : Lemma
+  (ensures (
+    let n = monomial 64 in
+    let a = of_vec128 p in
+    let a0 = mod (shift (mod a n) (v s)) n in
+    let a1 = mod (shift (div a n) (v s)) n in
+    cast U128 1 (vec_shift_left (cast U64 2 p) s) ==
+      to_vec128 (add (shift a1 64) a0)
+  ))
+
+val lemma_vec128_shift_right_64 (p:vec128) (s:shiftval U64) : Lemma
+  (ensures (
+    let n = monomial 64 in
+    let a = of_vec128 p in
+    let a0 = mod (shift (mod a n) (-(v s))) n in
+    let a1 = mod (shift (div a n) (-(v s))) n in
+    cast U128 1 (vec_shift_right (cast U64 2 p) s) ==
+      to_vec128 (add (shift a1 64) a0)
   ))
