lib/Lib.IntVector.fsti
@@ -16,7 +16,6 @@ inline_for_extraction
 val vec_t: t:v_inttype -> w:width -> Type0
 
 val reveal_vec_1: t:v_inttype -> Lemma
-  (requires t <> U128)
   (ensures vec_t t 1 == sec_int_t t)
 
 inline_for_extraction
@@ -43,7 +42,6 @@ val vecv_extensionality: #t:v_inttype -> #w:width -> f1:vec_t t w -> f2:vec_t t 
   (ensures f1 == f2)
 
 val reveal_vec_v_1: #t:v_inttype -> f:vec_t t 1 -> Lemma
-  (requires t <> U128)
   (ensures (
     reveal_vec_1 t;
     f == index (vec_v f) 0))
@@ -258,6 +256,15 @@ val vec_shift_right_uint128_small2: v1:vec_t U64 4 -> s:shiftval U128{uint_v s %
       ((vec_v v1).[1] >>. s)
      (((vec_v v1).[2] >>. s) |. ((vec_v v1).[3] <<. (64ul -! s)))
       ((vec_v v1).[3] >>. s))
+
+val vec_cast_uint128: v1:vec_t U128 1 -> Lemma
+  (vec_v (cast U64 2 v1) == create2
+     (to_u64 (vec_v v1).[0])
+     (to_u64 ((vec_v v1).[0] >>. 64ul)))
+
+val vec_cast_2_uint64: v1:vec_t U64 2 -> Lemma
+  (vec_v (cast U128 1 v1) == create 1
+     (((to_u128 (vec_v v1).[1]) <<. 64ul) +! (to_u128 (vec_v v1).[0])))
 
 inline_for_extraction
 val vec_rotate_right_lanes: #t:v_inttype -> #w:width
